Knapsack revisited

examples/Knapsack.v
@@ -35,7 +35,7 @@ Section MemoTable.
   Instance Memo : Cont MemoShape MemoPos
     := { valid := valid \o pair (snd \o fst) snd }.
 
-  Definition Table := GFix Memo.
+  Definition Table := LFix Memo.
 
   Definition ConsT (x : A * App G Table)
     : App Memo Table :=
@@ -58,9 +58,9 @@ Section MemoTable.
   Definition Cons : A * App G Table ~> App Memo Table
     := Eval unfold ConsT in MkMorph ConsT_morph.
 
-  Definition headT_ (t : Table) : A := fst (shape (g_out t)).
+  Definition headT_ (t : Table) : A := fst (shape (l_out t)).
   Definition tailT_ (t : Table) : App G Table :=
-    match g_out t with
+    match l_out t with
     | {| shape := (a, st); cont := kt |} =>
         {| shape := st; cont := fun e =>
                                   match e with
@@ -71,24 +71,30 @@ Section MemoTable.
   Lemma headT_morph : forall x y, x =e y -> headT_ x =e headT_ y.
   Proof.
     intros x y Exy.
-    unfold headT_. apply GFixR_unfold in Exy. destruct Exy as [Sxy Kxy].
-    replace (GFix_out x) with (g_out x) in * by reflexivity.
-    replace (GFix_out y) with (g_out y) in * by reflexivity.
-    destruct (g_out x) as [sx kx], (g_out y) as [sy ky]. simpl in *.
-    destruct sx as [ax tx], sy as [ay ty], Sxy as [Sxy _]; simpl in *; trivial.
+    destruct x as [[[a sx] kx]], y as [[[b sy] ky]]. simpl in *.
+    unfold headT_. simpl. destruct Exy as [[]]. trivial.
+    (* unfold headT_. apply GFixR_unfold in Exy. destruct Exy as [Sxy Kxy]. *)
+    (* replace (GFix_out x) with (g_out x) in * by reflexivity. *)
+    (* replace (GFix_out y) with (g_out y) in * by reflexivity. *)
+    (* destruct (g_out x) as [sx kx], (g_out y) as [sy ky]. simpl in *. *)
+    (* destruct sx as [ax tx], sy as [ay ty], Sxy as [Sxy _]; simpl in *; trivial. *)
   Qed.
   Definition headT := Eval unfold headT_ in MkMorph headT_morph.
 
   Lemma tailT_morph : forall x y, x =e y -> tailT_ x =e tailT_ y.
   Proof.
     intros x y Exy.
-    unfold tailT_. apply GFixR_unfold in Exy. destruct Exy as [Sxy Kxy].
-    replace (GFix_out x) with (g_out x) in * by reflexivity.
-    replace (GFix_out y) with (g_out y) in * by reflexivity.
-    destruct (g_out x) as [sx kx], (g_out y) as [sy ky]. simpl in *.
-    destruct sx as [ax tx], sy as [ay ty], Sxy as [_ Sxy]; simpl in *; trivial.
-    constructor; trivial; simpl.
-    intros [v1 V1] [v2 V2] Ev. simpl in *; subst. apply Kxy. trivial.
+    destruct x as [[[a sx] kx]], y as [[[b sy] ky]]. simpl in *.
+    unfold tailT_. simpl. destruct Exy as [[]]. constructor; trivial.
+    simpl. intros [v1 V1] [v2 V2]; simpl. intros Eq; subst.
+    apply H2. trivial.
+    (* unfold tailT_. apply GFixR_unfold in Exy. destruct Exy as [Sxy Kxy]. *)
+    (* replace (GFix_out x) with (g_out x) in * by reflexivity. *)
+    (* replace (GFix_out y) with (g_out y) in * by reflexivity. *)
+    (* destruct (g_out x) as [sx kx], (g_out y) as [sy ky]. simpl in *. *)
+    (* destruct sx as [ax tx], sy as [ay ty], Sxy as [_ Sxy]; simpl in *; trivial. *)
+    (* constructor; trivial; simpl. *)
+    (* intros [v1 V1] [v2 V2] Ev. simpl in *; subst. apply Kxy. trivial. *)
   Qed.
   Definition tailT := Eval unfold tailT_ in MkMorph tailT_morph.
 End MemoTable.
@@ -99,54 +105,42 @@ Arguments tailT {Sg}%type_scope {Esh} {Pg}%type_scope {G} {A}%type_scope {H}.
 
 Definition dyna `{setoid A} `{setoid B} `{C : Cont Sc Pc}
   (a : App C (Table C A) ~> A) (c : RCoalg C B) : B ~> A
-  := headT \o hylo (g_in \o Cons \o pair a id) c.
+  := headT \o hylo (l_in \o Cons \o pair a id) c.
 
 Definition NatF := Sum (K unit) Id.
 
 Lemma valid_inr_tt : valid (Cont:=NatF) (inr tt, inr tt).
 Proof. reflexivity. Qed.
-Fixpoint lookupT_ (x : nat) (t : Table NatF int) {struct x}: option int :=
+Fixpoint lookupT (x : nat) (t : Table NatF int) {struct x}: option int :=
   match x with
-  | 0 => Some (headT t)
+  | 0 => Some (headT_ t)
   | S y =>
-      match tailT t with
+      match tailT_ t with
       | MkCont st kt =>
           match st with
           | inl tt => fun _ => None
-          | inr tt => fun k => lookupT_ y (k (MkElem (inr tt) valid_inr_tt))
+          | inr tt => fun k => lookupT y (k (MkElem (inr tt) valid_inr_tt))
           end kt
       end
   end.
 
 Lemma lookupT_morph
-  : forall x y, x =e y -> lookupT_ (fst x) (snd x) =e lookupT_ (fst y) (snd y).
+  : forall x y, x =e y -> forall t t',  t =e t' -> lookupT x t =e lookupT y t'.
 Proof.
-  intros [x t] [y t'] [Exy Et]. simpl in *. subst. revert t t' Et.
+  intros x y Exy; simpl in Exy. subst.
   induction y as [|y Ih]; intros t t' Rt.
-  - simpl in *. apply GFixR_unfold in Rt. destruct Rt as [St Kt].
-    revert St Kt. replace (GFix_out t) with (g_out t) in * by reflexivity.
-    replace (GFix_out t') with (g_out t') in * by reflexivity. intros St Kt.
-    destruct (g_out t) as [[a st] kt], (g_out t') as [[b st'] kt']; simpl in *.
-    destruct St;subst; trivial.
-  - simpl. apply GFixR_unfold in Rt. revert Rt.
-    replace (GFix_out t) with (g_out t) in * by reflexivity.
-    replace (GFix_out t') with (g_out t') in * by reflexivity.
-    destruct (g_out t) as [[a st] kt], (g_out t') as [[b st'] kt']; simpl in *.
-    intros [[Sab St] Kt].
+  - simpl. f_equal. cut (headT_ t =e headT_ t');  try trivial.
+    apply headT_morph. trivial.
+  - simpl. assert (Tt : tailT_ t =e tailT_ t') by (apply tailT_morph; trivial).
+    clear Rt. destruct tailT_ as [st kt], tailT_ as [st' kt'].
+    destruct Tt as [St Kt]. simpl in *.
     destruct st as [[]|[]], st' as [[]|[]];
       try discriminate; try destruct St; trivial.
-    subst. apply Ih, Kt. trivial.
+    apply Ih, Kt. trivial.
 Qed.
 
-Definition lookupT : nat * Table NatF int ~> option int
-  := MkMorph lookupT_morph.
-
-Definition lookup_memo : Ext lookupT.
-  calculate.
-unfold lookupT, lookupT_.
-simpl.
-reflexivity.
-Defined.
+(* Definition lookupT : nat * Table NatF int ~> option int *)
+(*   := MkMorph lookupT_morph. *)
 
 Definition out_nat : nat ~> App NatF nat.
 |{ n ~>
@@ -175,23 +169,23 @@ Fixpoint memo_knapsack table wvs :=
   match wvs with
   | nil => nil
   | h :: t =>
-      match target lookup_memo (Nat.pred (fst h), table) with
+      match lookupT (Nat.pred (fst h)) table with
       | Some u => (u + snd h)%sint63 :: memo_knapsack table t
       | None => memo_knapsack table t
       end
   end.
 
 Lemma memo_knapsack_morph wvs :
-  forall t1 t2, GFixR t1 t2 -> memo_knapsack t1 wvs = memo_knapsack t2 wvs.
+  forall t1 t2, LFixR t1 t2 -> memo_knapsack t1 wvs = memo_knapsack t2 wvs.
 Proof.
   intros t1 t2 Rt.
   (* Opaque lookupT lookupT_. *)
   induction wvs; simpl; trivial.
   destruct a as [n i]; simpl.
-  assert (RWt : lookupT (Nat.pred n, t1) =e lookupT (Nat.pred n, t2))
-    by (apply app_eq; simpl; split; trivial).
-  simpl. rewrite RWt. clear RWt Rt. unfold lookupT, lookupT_. simpl.
-  destruct (lookupT_ _); simpl; try rewrite IHwvs; reflexivity.
+  assert (RWt : lookupT (Nat.pred n) t1 =e lookupT (Nat.pred n) t2)
+    by (apply lookupT_morph; simpl; trivial).
+  simpl. rewrite RWt. clear RWt Rt.
+  destruct lookupT; simpl; try rewrite IHwvs; reflexivity.
   (* Transparent lookupT lookupT_. *)
 Qed.
 
@@ -212,7 +206,7 @@ Lemma knapsack_alg_morph wvs
 Proof.
   intros [sx kx] [sy ky] [Es Ek]. simpl in *.
   destruct sx as [[]|[]], sy as [[]|[]]; try destruct Es; trivial.
-  assert (RR : GFixR (kx (MkElem (inr tt) valid_inr_tt))
+  assert (RR : LFixR (kx (MkElem (inr tt) valid_inr_tt))
                  (ky (MkElem (inr tt) valid_inr_tt)))
     by (apply Ek; trivial).
   rewrite (memo_knapsack_morph wvs RR).
@@ -225,7 +219,9 @@ Definition knapsackA (wvs : list (nat * int))
 
 Example ex1 wvs : Ext (dyna (knapsackA wvs) out_nat).
 calculate.
-unfold dyna, headT, fst, g_in, Cons, pair, out_nat, knapsackA.
+unfold dyna, fst, g_in, Cons, pair, out_nat, knapsackA, headT, tailT.
+unfold comp, fst, snd, pair, valid, id, GFix_out.
+unfold hylo, lookupT, headT_, tailT_.
 simpl.
 reflexivity.
 Defined.
@@ -234,6 +230,18 @@ Module ToExtract.
   Definition knapsack := Eval unfold ex1 in ex1.
 End ToExtract.
 
-Extraction Inline app.
+Require ExtrOcamlNatInt.
+Extraction Inline LFix_out.
+Extraction Inline shape.
+Extraction Inline headT_.
+Extraction Inline tailT_.
+Extraction Inline l_out.
+Extraction Inline LFix_out.
+Extraction Inline Memo.
+Extraction Inline fst.
+Extraction Inline snd.
+Extraction Inline pair.
+Extraction Inline Morphism.app.
+Extraction Inline Nat.pred.
 Set Extraction Flag 2047.
 Recursive Extraction ToExtract.
